ironfleet/ravana/RefinementProof/ControllerRecvEvent.dfy
@@ -1,0 +1,174 @@
+include "../Types.i.dfy"
+include "../Refinement.i.dfy"
+include "../Service.i.dfy"
+include "../DistributedSystem.i.dfy"
+include "../RefinementLemmas.i.dfy"
+
+module Refinement_Proof_ControllerRecvEvent {
+  import opened Types_i
+  import opened Refinement_i
+  import opened Service_i
+  import opened DistributedSystem_i
+  import opened RefinementLemmas_i
+
+  predicate conditions(rs: RState, rs': RState)
+  {
+    rstate_valid(rs)
+
+    && LEnvironment_Next(rs.environment, rs'.environment)
+    && rs.environment.nextStep.LEnvStepHostIos?
+    && rs.endpoint_logger == rs'.endpoint_logger
+    && rs.initControllerState == rs'.initControllerState
+    && rs.environment.nextStep.actor in rs.server_controllers
+    && rs.environment.nextStep.actor in rs'.server_controllers
+    && Node_ControllerRecvEvent(
+                rs.server_controllers[rs.environment.nextStep.actor],
+                rs'.server_controllers[rs.environment.nextStep.actor],
+                rs.environment.nextStep.ios)
+    && rs.server_switches == rs'.server_switches
+    && rs.server_logger == rs'.server_logger
+    && rs'.server_controllers == rs.server_controllers[
+        rs.environment.nextStep.actor := rs'.server_controllers[rs.environment.nextStep.actor]]
+  }
+
+  lemma lemma_refines_ControllerRecvEvent(rs: RState, rs': RState)
+  requires conditions(rs, rs')
+  ensures rstate_valid(rs')
+  ensures refinement(rs) == refinement(rs')
+  {
+    lemma_packets_are_valid(rs, rs');
+
+    lemma_recved_events_valid(rs, rs');
+
+    assert refinement_switchStates(rs.server_switches)
+        == refinement_switchStates(rs'.server_switches);
+
+    assert refinement_controllerState(rs.server_logger.log, rs.initControllerState)
+        == refinement_controllerState(rs'.server_logger.log, rs'.initControllerState);
+
+    assert refinement_outstandingCommands(rs.server_logger.log, rs.initControllerState, rs.server_switches)
+        == refinement_outstandingCommands(rs'.server_logger.log, rs'.initControllerState, rs'.server_switches);
+
+    assert refinement_outstandingEvents(rs.server_switches, rs.server_logger.log)
+        == refinement_outstandingEvents(rs'.server_switches, rs'.server_logger.log);
+  }
+
+  lemma lemma_recved_events_valid(rs: RState, rs': RState)
+  requires conditions(rs, rs')
+  ensures controllers_recved_events_valid(rs'.server_switches, rs'.server_controllers)
+  {
+    forall cn | cn in rs'.server_controllers
+    ensures 
+      forall sip :: sip in rs'.server_controllers[cn].recved_events ==>
+        sip.switch in rs'.server_switches &&
+        sip.event_id in rs'.server_switches[sip.switch].bufferedEvents &&
+        rs'.server_switches[sip.switch].bufferedEvents[sip.event_id] == rs'.server_controllers[cn].recved_events[sip]
+    {
+      forall sip | sip in rs'.server_controllers[cn].recved_events
+      ensures sip.switch in rs'.server_switches
+      ensures sip.event_id in rs'.server_switches[sip.switch].bufferedEvents
+      ensures rs'.server_switches[sip.switch].bufferedEvents[sip.event_id]
+           == rs'.server_controllers[cn].recved_events[sip]
+      {
+        lemma_recved_event_valid(rs, rs', cn, sip);
+        
+      }
+    }
+    reveal_controllers_recved_events_valid();
+  }
+
+  lemma lemma_recved_event_valid(rs: RState, rs': RState, cn: EndPoint, sip: SwitchIdPair)
+  requires conditions(rs, rs')
+  requires cn in rs'.server_controllers
+  requires sip in rs'.server_controllers[cn].recved_events
+  ensures sip.switch in rs'.server_switches
+  ensures sip.event_id in rs'.server_switches[sip.switch].bufferedEvents
+  ensures rs'.server_switches[sip.switch].bufferedEvents[sip.event_id]
+       == rs'.server_controllers[cn].recved_events[sip]
+  {
+    if (cn == rs.environment.nextStep.actor) {
+      var recv_packet := rs.environment.nextStep.ios[0].r;
+      if (sip == SwitchIdPair(recv_packet.src, recv_packet.msg.event_id)) {
+        lemma_event_msg_is_valid(rs, rs');
+        assert rs.environment.nextStep.ios[0].r.src == sip.switch;
+        assert rs.environment.nextStep.ios[0].r.msg.event ==
+            rs'.server_controllers[cn].recved_events[sip];
+        assert rs.environment.nextStep.ios[0].r.msg.event_id == sip.event_id;
+      } else {
+        assert sip in rs.server_controllers[cn].recved_events;
+        reveal_controllers_recved_events_valid();
+        assert sip.switch in rs.server_switches;
+        assert sip.event_id in rs.server_switches[sip.switch].bufferedEvents;
+        assert rs.server_switches[sip.switch].bufferedEvents[sip.event_id]
+             == rs.server_controllers[cn].recved_events[sip];
+      }
+    } else {
+      reveal_controllers_recved_events_valid();
+      assert sip.switch in rs.server_switches;
+      assert sip.event_id in rs.server_switches[sip.switch].bufferedEvents;
+      assert rs.server_switches[sip.switch].bufferedEvents[sip.event_id]
+           == rs.server_controllers[cn].recved_events[sip];
+    }
+  }
+
+  lemma lemma_event_msg_is_valid(rs: RState, rs': RState)
+  requires conditions(rs, rs')
+  ensures is_valid_EventMessage(rs,
+      rs.environment.nextStep.ios[0].r.src,
+      rs.environment.nextStep.ios[0].r.dst,
+      rs.environment.nextStep.ios[0].r.msg)
+  {
+    reveal_packets_are_valid();
+  }
+
+  lemma lemma_packets_are_valid(rs: RState, rs': RState)
+  requires conditions(rs, rs')
+  ensures packets_are_valid(rs')
+  {
+    packet_validation_preservation(rs, rs');
+    lemma_packets_are_valid_no_sending(rs, rs');
+  }
+
+  lemma packet_validation_preservation(rs: RState, rs': RState)
+  requires conditions(rs, rs')
+  ensures packet_validation_preserved(rs, rs')
+  {
+    forall p : LPacket<EndPoint, RavanaMessage>
+    ensures 
+        is_valid_message(rs, p.src, p.dst, p.msg) ==>
+        is_valid_message(rs', p.src, p.dst, p.msg)
+    {
+      if (is_valid_message(rs, p.src, p.dst, p.msg)) {
+        match p.msg
+          case EventMessage(event: Event, event_id: int) => {
+            assert is_valid_EventMessage(rs', p.src, p.dst, p.msg);
+          }
+          case EventAck(event_ack_id: int) => {
+            assert is_valid_EventAck(rs', p.src, p.dst, p.msg);
+          }
+          case CommandMessage(command: Command, command_id: int) => {
+            assert is_valid_CommandMessage(rs', p.src, p.dst, p.msg);
+          }
+          case CommandAck(command_ack_id: int) => {
+            assert is_valid_CommandAck(rs', p.src, p.dst, p.msg);
+          }
+          case InitNewMaster(leader_id: int) => {
+            assert is_valid_InitNewMaster(rs', p.src, p.dst, p.msg);
+          }
+          case NewMaster(master_id: int) => {
+            assert is_valid_NewMaster(rs', p.src, p.dst, p.msg);
+          }
+          case NewMasterAck => {
+            assert is_valid_NewMasterAck(rs', p.src, p.dst, p.msg);
+          }
+          case LogMessage(log_entry: LogEntry) => {
+            assert is_valid_LogMessage(rs', p.src, p.dst, p.msg);
+          }
+          case LogBroadcastMessage(full_log: seq<LogEntry>) => {
+            assert is_valid_LogBroadcastMessage(rs', p.src, p.dst, p.msg);
+          }
+      }
+    }
+    reveal_packet_validation_preserved();
+  }
+}
